Implement Smart STOREI

Uppaal_Networks/UPPAAL_Asm.thy
@@ -57,7 +57,8 @@ fun step :: "instr \<Rightarrow> state \<Rightarrow> state option" where
      else None)" |
   "step STORE (pc, v # r # st, m, f, rs) =
     (if r \<ge> 0 \<and> nat r < length m then Some (pc + 1, st, m[nat r := v], f, rs) else None)" |
-  "step (STOREI r v) (pc, st, m, f, rs) = Some (pc + 1, st, m[r := v], f, rs)" |
+  "step (STOREI r v) (pc, st, m, f, rs) =
+    (if r < length m then Some (pc + 1, st, m[r := v], f, rs) else None)" |
   "step COPY (pc, st, m, f, rs) = Some (pc + 1, int_of f # st, m, f, rs)" |
   "step CALL (pc, q # st, m, f, rs) =
     (if q \<ge> 0 then Some (nat q, int pc # st, m, f, rs) else None)" |
